src/Language/PlutusIR/Transform/Inline/DecOpt.v
@@ -1,0 +1,111 @@
+From PlutusCert Require Import
+  Util.List
+  Util.DecOpt
+  Language.PlutusIR
+  Language.PlutusIR.DecOpt
+  Language.PlutusIR.Transform.Inline
+  Language.PlutusIR.Analysis.Equality.DecOpt.
+
+From QuickChick Require Import QuickChick.
+From CTProxy Require Import CTProxy.
+
+
+
+
+QCDerive EnumSized for binder_info.
+
+Instance Dec_eq_binder_info : Dec_Eq binder_info.
+Proof.
+  constructor.
+  unfold ssrbool.decidable.
+  decide equality.
+  - apply Dec_eq_Term.
+  - apply Dec_eq_Ty.
+Qed.
+
+Instance Dec_eq_ctx : Dec_Eq ctx.
+Proof.
+  apply Dec_eq_list.
+  apply Dec_eq_prod.
+  - apply Dec_eq_string.
+  - apply Dec_eq_binder_info.
+Qed.
+
+
+
+
+
+
+
+MetaCoq Run (deriveCTProxy inline).
+
+Local Hint Constructors 
+  inline 
+  inline_Bindings_Rec 
+  inline_Bindings_NonRec 
+  inline_Binding 
+  inline_Ty 
+  inline_Var
+    : inline_hints. 
+
+Lemma inline_proxy_sound : inline_proxy_sound_type.
+Proof. deriveCTProxy_sound inline_hints. Qed.
+
+
+
+
+
+QCDerive DecOpt for (inline_proxy tag).
+
+Instance DecOptinline_proxy_sound tag : DecOptSoundPos (inline_proxy tag).
+Proof. (* derive_sound. Qed. *) idtac "Admitted: DecOptinline_proxy_sound". Admitted.
+
+
+
+(* inline *)
+
+Instance DecOptinline c1 c2 tm : DecOpt (inline c1 c2 tm) :=
+{| decOpt s := @decOpt (inline_proxy (inline_tag c1 c2 tm)) (DecOptinline_proxy (inline_tag c1 c2 tm)) s |}.
+
+Instance DecOptinline_sound c1 c2 tm : DecOptSoundPos (inline c1 c2 tm).
+Proof. derive__sound (inline_proxy_sound (inline_tag c1 c2 tm)). Qed.
+
+
+
+(* inline_Bindings_Rec *)
+
+Instance DecOptinline_Bindings_Rec c1 c2 tm : DecOpt (inline_Bindings_Rec c1 c2 tm) :=
+{| decOpt s := @decOpt (inline_proxy (inline_Bindings_Rec_tag c1 c2 tm)) (DecOptinline_proxy (inline_Bindings_Rec_tag c1 c2 tm)) s |}.
+
+Instance DecOptinline_Bindings_Rec_sound c1 c2 tm : DecOptSoundPos (inline_Bindings_Rec c1 c2 tm).
+Proof. derive__sound (inline_proxy_sound (inline_Bindings_Rec_tag c1 c2 tm)). Qed.
+
+
+
+(* inline_Bindings_NonRec *)
+
+Instance DecOptinline_Bindings_NonRec c1 c2 tm : DecOpt (inline_Bindings_NonRec c1 c2 tm) :=
+{| decOpt s := @decOpt (inline_proxy (inline_Bindings_NonRec_tag c1 c2 tm)) (DecOptinline_proxy (inline_Bindings_NonRec_tag c1 c2 tm)) s |}.
+
+Instance DecOptinline_Bindings_NonRec_sound c1 c2 tm : DecOptSoundPos (inline_Bindings_NonRec c1 c2 tm).
+Proof. derive__sound (inline_proxy_sound (inline_Bindings_NonRec_tag c1 c2 tm)). Qed.
+
+
+
+(* inline_Binding *)
+
+Instance DecOptinline_Binding c1 c2 tm : DecOpt (inline_Binding c1 c2 tm) :=
+{| decOpt s := @decOpt (inline_proxy (inline_Binding_tag c1 c2 tm)) (DecOptinline_proxy (inline_Binding_tag c1 c2 tm)) s |}.
+
+Instance DecOptinline_Binding_sound c1 c2 tm : DecOptSoundPos (inline_Binding c1 c2 tm).
+Proof. derive__sound (inline_proxy_sound (inline_Binding_tag c1 c2 tm)). Qed.
+
+
+
+(* inline_Ty *)
+
+Instance DecOptinline_Ty c1 c2 tm : DecOpt (inline_Ty c1 c2 tm) :=
+{| decOpt s := @decOpt (inline_proxy (inline_Ty_tag c1 c2 tm)) (DecOptinline_proxy (inline_Ty_tag c1 c2 tm)) s |}.
+
+Instance DecOptinline_Ty_sound c1 c2 tm : DecOptSoundPos (inline_Ty c1 c2 tm).
+Proof. derive__sound (inline_proxy_sound (inline_Ty_tag c1 c2 tm)). Qed.
